\documentclass[letterpaper,fleqn]{article}

\usepackage{amsmath}
\usepackage{amssymb}
\usepackage[letterpaper, margin=1in]{geometry}
%\usepackage{xcolor, colortbl}
%\usepackage{cancel}
%\usepackage{tabularx}
\usepackage{blkarray}
\usepackage{mathtools}
\usepackage{enumerate}

%\setlength{\extrarowheight}{3pt}

\begin{document}
	\newcommand{\sect}[2]{
		\noindent\textbf{Section #1}
		\begin{enumerate}
			#2
		\end{enumerate}
	}
	
	\newcommand{\ques}[3][\quad] {
%		\fbox{
		\begin{minipage}{\textwidth}
			\item [#2.] #1
			#3
		\end{minipage}\\
%		}
	}
	
	\sect{2.4}{
		\ques{1}{
			\begin{enumerate}[(a)]
				\item 
				$\textbf{I}^2=\textbf{I}$
				\item 
				$\textbf{1} \cdot \textbf{1}=n$
				\item 
				$\textbf{I1}=\textbf{1}$
				\item 
				$\textbf{Ie}_i=\textbf{e}_i$
				\item 
				$\textbf{1} \cdot \textbf{e}_i=1$
				\item 
				$\textbf{e}_i \cdot \textbf{e}_i=1$
				\item 
				$\textbf{e}_i \cdot \textbf{e}_j=0$
				\item 
				$\textbf{1I1}=\textbf{1} \cdot \textbf{1}=n$
				\item 
				$\textbf{e}_i\textbf{Ie}_j=\textbf{e}_i \cdot \textbf{e}_j=0$
			\end{enumerate}
		}	
		
		\ques{2}{
			\begin{enumerate}[(a)]
				\item 
				$\begin{bmatrix*}[r]
					3 & 5 & 7 \\
					2 & -1 & 1 \\
					1 & 6 & -2 \\
				\end{bmatrix*}
				\begin{bmatrix}
					x_1 \\ x_2 \\ x_3 \\
				\end{bmatrix}
				=
				\begin{bmatrix}
					8 \\ 4 \\ 6 \\	
				\end{bmatrix}$
				\item 
				$\begin{bmatrix*}[r]
					3 & 5 & 7 & -8 \\
					2 & -1 & 1 & -4 \\
					1 & 6 & -2 & -6 \\
				\end{bmatrix*}
				\begin{bmatrix}
					x_1 \\ x_2 \\ x_3 \\ 1 \\
				\end{bmatrix}
				=
				\begin{bmatrix}
					0 \\ 0 \\ 0 \\
				\end{bmatrix}$
			\end{enumerate}
		}
		
		
		\ques{6}{
			\begin{enumerate}
				\item [(a)]
				$\textbf{p'}=
				\underbrace{\begin{bmatrix*}[r]
						1.5 & -0.2 \\
						0.3 & 0.9 \\
				\end{bmatrix*}}_{\textbf{A}}\textbf{p}+
				\underbrace{\begin{bmatrix}
						100 \\ 50 \\
				\end{bmatrix}}_{\textbf{B}}$
				\item [(c)]
				$\begin{aligned}[t]
					\textbf{p"} &= \textbf{A}(\textbf{Ap}+\textbf{B})+\textbf{B} \\ 
					&= \textbf{A}^2\textbf{p}+(\textbf{A}+\textbf{I})\textbf{B} \\
				\end{aligned}$ \\
				$\begin{aligned}[t]
					\textbf{p}^{(3)} &= \textbf{A}(\textbf{A}^2\textbf{p}+(\textbf{A}+\textbf{I})\textbf{B})+\textbf{B} \\ 
					&= \textbf{A}^3\textbf{p}+(\textbf{A}(\textbf{A}+\textbf{I})+\textbf{I})\textbf{B} \\
					&= \textbf{A}^3\textbf{p}+(\textbf{A}^2+\textbf{A}+\textbf{I})\textbf{B} \\
				\end{aligned}$ \\
			\end{enumerate}
		}
		
		\ques[{$\textbf{Ax}=\textbf{By}=[1,1]$, $\textbf{Ay}=[1,0]$, $\textbf{Bx}=[0,1]$}]{10}{
			\begin{enumerate}
				\item [(c)]
				$\begin{aligned}[t]
					\textbf{z} &= (\textbf{A}+\textbf{B})\textbf{x}-2(\textbf{A}+\textbf{B})\textbf{y} \\
					&= \textbf{Ax}+\textbf{Bx}-2\textbf{Ay}-2\textbf{By} \\
					&= [1,1]+[0,1]-2[1,0]-2[1,1] \\
					&= [-3,0] \\
				\end{aligned}$
				\item [(d)]
				$\begin{aligned}[t]
					\textbf{z} &= (3\textbf{A}+\textbf{B})(\textbf{x}+\textbf{y}) \\
					&= 3\textbf{Ax}+3\textbf{Ay}+\textbf{Bx}+\textbf{By} \\
					&= 3[1,1]+3[1,0]+[0,1]+[1,1] \\
					&= [7,5] \\
				\end{aligned}$
			\end{enumerate}
		}
	}	
	
	\newpage
	
	\sect{2.5}{
		\ques{2}{
			\begin{enumerate}[(a)]
				\item
				$|[1,1,1]|_e=\sqrt{3}$,\\ $|[1,1,1]|_s=3$,\\ $|[1,1,1]|_{mx}=1$ \\
			\end{enumerate}
		}
		
		\ques{10}{
			\begin{enumerate}[(a)]
				\item 
				$\textbf{A}=\begin{bmatrix}
					1.3 & -0.1 & -0.2 \\
					0.4 & 0.8 & -0.3 \\
					0.1 & 0.1 & 1.1 \\
				\end{bmatrix}$ \\
				$\|\textbf{A}\|_s=1.8$, $\|\textbf{A}\|_{mx}=1.6$
				\item
				$\textbf{p'}=\textbf{Ap}$, $\textbf{p}=[10,10,10]$ \\
				$|\textbf{p'}|_s\leq(1.8|\textbf{p}|_s=54)$, $|\textbf{p'}|_{mx}\leq(1.6|\textbf{p}|_{mx}=16)$ \\
				$\textbf{p'}=[10,9,13]$ \\
				$|\textbf{p'}|_s=32$, $|\textbf{p'}|_{mx}=13$		
			\end{enumerate}
		}
		
		\ques{26}{
			\begin{enumerate}
				\item [(c)]
				$\textbf{A}=\begin{bmatrix*}[r]
					1 & 6 \\
					-2 & -6 \\
				\end{bmatrix*}$, $\textbf{u}_1=[-2,1]$, $\textbf{u}_2=[-3,2]$ \\
				$\textbf{Au}_1=\lambda_1\textbf{u}_1$ \\
				$\textbf{Au}_1=[4,-2]=-2\textbf{u}_1$, $\lambda_1=-2$ \\
				$\textbf{Au}_2=\lambda_2\textbf{u}_2$ \\
				$\textbf{Au}_2=[9,-6]=-3\textbf{u}_2$, $\lambda_2=-3$
			\end{enumerate}
		}
		
		\ques{28}{
			\begin{enumerate}
				\item [(c)]
				$\textbf{u}_1=[1,1]$, $\textbf{u}_2=[-5,6]$ \\
				$\lambda_1=7$, $\lambda_2=-4$ \\
				$\textbf{v}=7\textbf{u}_1+\textbf{u}_2$ \\
				$\begin{aligned}[t]
					\textbf{A}^3\textbf{v} &= \textbf{A}^3(7\textbf{u}_1+\textbf{u}_2) \\
					&= 7\textbf{A}^3\textbf{u}_1+\textbf{A}^3\textbf{u}_2 \\
					&= 7(7^3)\textbf{u}_1+(-4)^3\textbf{u}_2 \\
					&= [7^4+4^3\cdot5, 7^4-4^3\cdot6]
				\end{aligned}$
			\end{enumerate}
		}
	}
	
	\sect{2.6}{
		\ques{6}{
			\begin{enumerate}
				\item [(b)]
				$G_2=\begin{bmatrix}
					0 & 1 & 1 & 1 & 1 & 0 & 0 & 0 \\
					1 & 0 & 1 & 1 & 0 & 0 & 0 & 0 \\
					1 & 1 & 0 & 1 & 0 & 0 & 0 & 0 \\
					1 & 1 & 1 & 0 & 0 & 0 & 0 & 1 \\ 
					1 & 0 & 0 & 0 & 0 & 1 & 1 & 1 \\
					0 & 0 & 0 & 0 & 1 & 0 & 1 & 1 \\ 
					0 & 0 & 0 & 0 & 1 & 1 & 0 & 1 \\
					0 & 0 & 0 & 1 & 1 & 1 & 1 & 0 \\
				\end{bmatrix}$ \\
				$\textbf{A}=\begin{bmatrix}
					0 & 1 & 1 & 1 \\
					1 & 0 & 1 & 1 \\
					1 & 1 & 0 & 1 \\
					1 & 1 & 1 & 0 \\
				\end{bmatrix}$, 
				$\textbf{B}=\begin{bmatrix}
					1 & 0 & 0 & 0 \\
					0 & 0 & 0 & 0 \\
					0 & 0 & 0 & 0 \\
					0 & 0 & 0 & 1 \\
				\end{bmatrix}$ \\
				$G_2=\begin{bmatrix}
					\textbf{A} & \textbf{B} \\
					\textbf{B} & \textbf{A} \\
				\end{bmatrix}$ \\
			\end{enumerate}
		}
		
		\ques[{
			$M=\begin{blockarray}{cc}
				& \text{From} \\
				\text{To} & 
				\begin{blockarray}{c*{8}{c}}
					& A & B & C & D & E & F & G & H \\
					\begin{block}{l[*{8}{c}]}
						A & 0 & 1/2 & 1/2 & 1/3 & 0 & 0 & 0 & 1/4 \\
						B & 1/4 & 0 & 0 & 1/3 & 0 & 0 & 0 & 0 \\
						C & 1/4 & 0 & 0 & 1/3 & 0 & 0 & 0 & 0 \\
						D & 1/4 & 1/2 & 1/2 & 0 & 0 & 0 & 0 & 0 \\
						E & 0 & 0 & 0 & 0 & 0 & 1/2 & 1/2 & 1/4 \\
						F & 0 & 0 & 0 & 0 & 1/3 & 0 & 0 & 1/4 \\
						G & 0 & 0 & 0 & 0 & 1/3 & 0 & 0 & 1/4 \\
						H & 1/4 & 0 & 0 & 0 & 1/3 & 1/2 & 1/2 & 0 \\
					\end{block}
				\end{blockarray}
			\end{blockarray} \\
			A=\begin{bmatrix}
				0 & 0 & 0 & 1/4 \\
				0 & 0 & 0 & 0 \\
				0 & 0 & 0 & 0 \\
				0 & 0 & 0 & 0 \\
			\end{bmatrix} \\
			M=\begin{bmatrix}
				\begin{bmatrix}
					0 & 1/2 & 1/2 & 1/3 \\
					1/4 & 0 & 0 & 1/3 \\
					1/4 & 0 & 0 & 1/3 \\
					1/4 & 1/2 & 1/2 & 0 \\
				\end{bmatrix} & A \\
				A^T & \begin{bmatrix}
					0 & 1/2 & 1/2 & 1/4 \\
					1/3 & 0 & 0 & 1/4 \\
					1/3 & 0 & 0 & 1/4 \\
					1/3 & 1/2 & 1/2 & 0 \\
				\end{bmatrix}
			\end{bmatrix}$
		}]{7}{}
	}
	
	\sect{3.1}{
		\ques{2}{
			\begin{enumerate}
				\item [(b)]
				$\underbrace{\begin{bmatrix*}[r]
					2 & -3 \\
					-5 & 6 \\
				\end{bmatrix*}}_A\begin{bmatrix}
					x \\ y \\
				\end{bmatrix}=
				\begin{bmatrix}
					5 \\ 10 \\
				\end{bmatrix}$ \\
				det$(A)=-3$ \\
				$x=\dfrac{\begin{vmatrix}
					5 & -3 \\
					10 & 6 \\
				\end{vmatrix}}{\text{det}(A)}$, 
				$y=\dfrac{\begin{vmatrix}
					2 & 5 \\
					-5 & 10 \\
				\end{vmatrix}}{\text{det}(A)}$ \\
			$x=\dfrac{60}{-3}$, $y=\dfrac{45}{-3}$ \\
			$x=-20$, $y=-15	$ \\
			\end{enumerate}
		}
		
		\ques{23}{
			\begin{enumerate}[(a)]
				\item \quad
				\begin{enumerate}
					\item [(i)]
					$\textbf{A}=\begin{bmatrix}
						4 & 0 \\
						2 & 2 \\
					\end{bmatrix}$ \\
					$\begin{aligned}[t]
						\text{det}(\textbf{A}-\lambda\textbf{I}) &= \begin{vmatrix}
							4-\lambda & 0 \\
							2 & 2-\lambda \\
						\end{vmatrix} \\
						&= (4-\lambda)(2-\lambda)-0\cdot2 \\
						&= (4-\lambda)(2-\lambda) \\
					\end{aligned}$ \\
					Eigenvalues are 4 and 2.
					
					
					\item [(iii)]
					$\textbf{A}=\begin{bmatrix}
						2 & 1 \\
						2 & 3 \\
					\end{bmatrix}$ \\
					$\begin{aligned}[t]
						\text{det}(\textbf{A}-\lambda\textbf{I}) &= \begin{vmatrix}
							2-\lambda & 1 \\
							2 & 3-\lambda \\
						\end{vmatrix} \\
						&= (2-\lambda)(3-\lambda)-1\cdot2 \\
						&= 6-5\lambda+\lambda^2-2\\
						&= \lambda^2-5\lambda+4 \\
						&= (\lambda-1)(\lambda-4) \\
					\end{aligned}$ \\
					Eigenvalues are 1 and 4.
				\end{enumerate}
			\end{enumerate}
		}
	}
\end{document}